\documentclass[12pt]{article}
\pagestyle{empty}
\title{Accompanied Definitions and Proofs}

\usepackage{fullpage,amssymb,amsmath,amsthm}

\newtheorem{definition}{Definition}
\newtheorem{lemma}{Lemma}


\begin{document}


subscript start from 0



\begin{definition} subseq(x, I) :=
\begin{itemize}
\item[•]subseq(x, I) := $\epsilon$ $\mid$ I = \{\}
\item[•]subseq(x, I) := subseq(x, I $\setminus$ i) $x_{i}$ where i = max(I) $\mid$ otherwise
\end{itemize}
\end{definition}


\begin{definition} shuffle(x, y) := \{ w $\mid$ w $\in$ perm(x y), subseq(w, A) = x, subseq(w, B) = y, A $\cap$ B = \{\}, A $\cup$ B = $Z_{|x|+|y|}$ \}
\begin{itemize}
\item[•]shuffle(x) := x
\item[•]shuffle(x, y) := \{ w $\mid$ w $\in$ perm(x y), subseq(w, A) = x, subseq(w, B) = y, A $\cap$ B = \{\}, A $\cup$ B = $Z_{|x|+|y|}$ \}
\item[•]shuffle($\cdots$, w) := $\bigcup_{W \in shuffle(\cdots)}$shuffle(W, w)
\end{itemize}
\end{definition}

\begin{lemma}
x $\in$ shuffle($\alpha_{0}^{W_{0}}$, $\cdots$) where $\mid x \mid_{\alpha_{i}}=W_{i}$ and $\bigcup\{ \alpha_{i} \} = \Sigma$
\end{lemma}

\begin{proof}[Proof by Mathematical Induction]$\vDash$

\subparagraph{Induction}
Assume x $\in$ shuffle($\alpha_{0}^{W_{0}}$, $\cdots$) where $\mid x \mid_{\alpha_{i}}=W_{i}$ and $\bigcup\{ \alpha_{i} \} = \Sigma$ for $\mid \Sigma \mid < k + 1$

\begin{itemize}
\item[•]Let x' $\in$ $\Sigma'$ where $\mid \Sigma \mid$ = k + 1, $\mid x' \mid_{\alpha_{i}}=W_{i}$ and $\bigcup\{ \alpha_{i} \} = \Sigma'$
\item[•]Let $I_{\alpha_{k}}$ = \{$ i \mid i \in Z_{k}, x'_{i} = \alpha_{k} $\}, $I_{\hat{\alpha_{k}}}$ = $Z_{\mid x \mid} \setminus I_{\alpha_{k}}$
\item[•]Let y = subseq(x, $I_{\hat{\alpha_{k}}}$) $\subseteq$ shuffle($\alpha_{0}^{W_{0}}$, $\cdots$, $\alpha_{k - 1}^{W_{k - 1}}$), y' = subseq(x, $I_{\alpha_{k}}$)
\item[•]Then y $\in$ shuffle($\alpha_{0}^{W_{0}}$, $\cdots$, $\alpha_{k - 1}^{W_{k - 1}}$)
\item[•]Since x' $\in$ shuffle(y, y'), x' $\in$ shuffle($\alpha_{0}^{W_{0}}$, $\cdots$)
\end{itemize}

\subparagraph{Baseline}
\begin{itemize}
\item[•]x $\in$ shuffle(x) = shuffle($\alpha_{0}^{W_{0}}$) where $\mid x \mid_{\alpha_{i}}=W_{i}$ and $\bigcup\{ \alpha_{i} \} = \Sigma$ for $\mid \Sigma \mid = 1$
\item[•]x $\in$ perm($\alpha_{0}^{W_{0}}$ $\alpha_{1}^{W_{1}}$) = shuffle($\alpha_{0}^{W_{0}}$, $\alpha_{1}^{W_{1}}$) where $\mid x \mid_{\alpha_{i}}=W_{i}$ and $\bigcup\{ \alpha_{i} \} = \Sigma$ for $\mid \Sigma \mid = 2$
\end{itemize}

\subparagraph{Conclusion}
x $\in$ shuffle($\alpha_{0}^{W_{0}}$, $\cdots$) where $\mid x \mid_{\alpha_{i}}=W_{i}$ and $\bigcup\{ \alpha_{i} \} = \Sigma$
\end{proof}

\begin{lemma}
shuffle(A B, C D) $\subseteq$ shuffle(A, C) shuffle(B, D)
\end{lemma}


\end{document}